\documentclass[12pt]{article}

\usepackage[margin=1in]{geometry}

\begin{document}
\thispagestyle{empty}

\noindent Using the definition of the \textbf{sigmoid function} we would have:

$$Pr\{A_t = a\} = \frac{e^{H_t(a)}}{e^{H_t(a)} + 1}$$
$$Pr\{A_t = b\} = 1 - Pr\{A_t = a\} = \frac{1}{e^{H_t(a)} + 1}$$

\noindent Extending the definition of the \textbf{soft-max distribution} for the case of two actions (k=2) we get the following:

$$Pr\{A_t=a\} = \frac{e^{H_t(a)}}{e^{H_t(a)} + e^{H_t(b)}}$$
$$Pr\{A_t=b\} = \frac{e^{H_t(b)}}{e^{H_t(a)} + e^{H_t(b)}}$$

\noindent According to the definition of the \textit{numerical preference}, if we substract an amount from each of the preferences
it does not affect the probabilities. So we can redifine $H_t(a)$ and $H_t(b)$ as:

$$H_t(b) \leftarrow  H_t(b) - H_t(b) = 0$$
$$H_t(a) \leftarrow  H_t(a) - H_t(b) = H_t(a)$$

\noindent and we get:

$$Pr\{A_t=a\} = \frac{e^{H_t(a)}}{e^{H_t(a)} + e^0} = \frac{e^{H_t(a)}}{e^{H_t(a)} + 1} $$
$$Pr\{A_t=b\} = \frac{e^{0}}{e^{H_t(a)} + e^{0}} = \frac{1}{e^{H_t(a)} + 1}$$

\end{document}
